tests/lean/run/linearNoConfusion.lean
@@ -9,11 +9,17 @@ from this file without updating that module's docstring.
 -/
 
 -- set_option debug.skipKernelTC true
+-- set_option trace.Meta.mkNoConfusion true
+-- set_option trace.Kernel true
+
+set_option genInjectivity false
 
 inductive Vec.{u} (α : Type) : Nat → Type u where
   | nil : Vec α 0
   | cons1 {n} : α → Vec α n → Vec α (n + 1)
   | cons2 {n} : α → Vec α n → Vec α (n + 1)
+
+#check Vec.cons1.noConfusion
 
 @[reducible] protected def Vec.noConfusionType'.{u_1, u} : {α : Type} →
   Sort u_1 → {a : Nat} → Vec.{u} α a → {a : Nat} → Vec α a → Sort u_1 :=
